classical logics don't need explicit efq

Cslib/Logics/Propositional/Defs.lean
@@ -105,7 +105,7 @@ abbrev IPL [Bot Atom] : Theory Atom :=
 
 /-- Classical logic further adds double negation elimination. -/
 abbrev CPL [Bot Atom] : Theory Atom :=
-  IPL ∪ Set.range (fun (A : Proposition Atom) ↦ ¬¬A → A)
+  Set.range (fun (A : Proposition Atom) ↦ ¬¬A → A)
 
 @[scoped grind]
 class IsIntuitionistic [Bot Atom] (T : Theory Atom) where
@@ -116,25 +116,18 @@ omit [DecidableEq Atom] in
 theorem isIntuitionisticIff [Bot Atom] (T : Theory Atom) : IsIntuitionistic T ↔ IPL ⊆ T := by grind
 
 @[scoped grind]
-class IsClassical [Bot Atom] (T : Theory Atom) extends IsIntuitionistic T where
+class IsClassical [Bot Atom] (T : Theory Atom) where
   dne (A : Proposition Atom) : (¬¬A → A) ∈ T
 
 omit [DecidableEq Atom] in
 @[scoped grind]
-theorem isClassicalIff [Bot Atom] (T : Theory Atom) : IsClassical T ↔ CPL ⊆ T := by
-  constructor
-  · grind
-  · intro _
-    have : IsIntuitionistic T := by grind
-    refine ⟨?_⟩
-    grind
+theorem isClassicalIff [Bot Atom] (T : Theory Atom) : IsClassical T ↔ CPL ⊆ T := by grind
 
 instance instIsIntuitionisticIPL [Bot Atom] : IsIntuitionistic (Atom := Atom) IPL where
   efq A := Set.mem_range.mpr ⟨A, rfl⟩
 
 instance instIsClassicalCPL [Bot Atom] : IsClassical (Atom := Atom) CPL where
-  efq A := Set.mem_union_left _ <| Set.mem_range.mpr ⟨A, rfl⟩
-  dne A := Set.mem_union_right _ <| Set.mem_range.mpr ⟨A, rfl⟩
+  dne A := Set.mem_range.mpr ⟨A, rfl⟩
 
 omit [DecidableEq Atom] in
 @[scoped grind]
@@ -144,7 +137,7 @@ theorem instIsIntuitionisticExtention [Bot Atom] {T T' : Theory Atom} [IsIntuiti
 omit [DecidableEq Atom] in
 @[scoped grind]
 theorem instIsClassicalExtention [Bot Atom] {T T' : Theory Atom} [IsClassical T] (h : T ⊆ T') :
-    IsClassical T' := by have :_ := instIsIntuitionisticExtention h; grind
+    IsClassical T' := by grind
 
 /-- Attach a bottom element to a theory `T`, and the principle of explosion for that bottom. -/
 @[reducible]
